Move code

proofmode/HTactics2.v
@@ -655,6 +655,146 @@ Section MODE.
   Unshelve. all: try exact 0.
   Qed.
 
+  Local Transparent APC.
+
+  Definition is_possibly_pure (fsp: fspec): Prop :=
+    exists x mn varg_src varg_tgt d r, fsp.(precond) x mn varg_src varg_tgt d r ∧ is_pure d
+  .
+
+  Definition stb_pure_incl (stb_tgt stb_src: string -> option fspec): Prop :=
+    forall fn fsp (FIND: stb_tgt fn = Some fsp) (PURE: is_possibly_pure fsp), stb_src fn = Some fsp
+  .
+
+  Local Transparent HoareCall.
+
+  Lemma hAPC_both
+        A (a0: shelve__ A) mp_src0 mp_tgt0 (mr_src0 mr_tgt0: Σ)
+        mn r rg
+        k_src k_tgt
+        _a (le: A -> A -> Prop)
+        (R: A -> Any.t -> Any.t -> iProp)
+        (eqr: Any.t -> Any.t -> Any.t -> Any.t -> Prop)
+        o_new_src o_new_tgt
+        o_src0 o_src1 o_tgt0 o_tgt1
+        (FUELS: o_src0 = Ord_S_n o_src1 5)
+        (FUELT: o_tgt0 = Ord_S_n o_tgt1 5)
+        ctx0
+        `{PreOrder _ le}
+
+        (* (WF: mk_wf R a0 ((Any.pair mp_src0 mr_src0↑), (Any.pair mp_tgt0 mr_tgt0↑))) *)
+
+        rx0
+        (* ips Xtra *)
+        (* (ACC: current_iPropL ctx0 ips) *)
+        (* (ENTAIL: bi_entails (from_iPropL ips) ((OwnT mr_tgt0) ** (Xtra ∧ Exactly rx))) *)
+        Xn Invtn Xtra
+        (ACC: current_iPropL ctx0 [(Invtn, OwnT mr_tgt0); (Xn, (Xtra ∧ Exactly rx0)%I)])
+        FR
+        (ENTAIL: bi_entails Xtra (R a0 mp_src0 mp_tgt0 ** FR))
+        (* (WFA: forall a1 mp_src1 mp_tgt1 (mr_src1 mr_tgt1: Σ) (INV: I mr_src1), *)
+        (*     mk_wf R a1 ((Any.pair mp_src1 mr_src1↑), (Any.pair mp_tgt1 mr_tgt1↑))) *)
+
+
+        stb_src stb_tgt d
+        (STBINCL: stb_pure_incl stb_tgt stb_src)
+        (ARG: forall
+            (mr_src1 mr_tgt1: Σ) (mp_src1 mp_tgt1 : Any.t) a1
+            (WLE: le a0 a1)
+            ctx1 rx1
+            (ACC: current_iPropL ctx1 [("INVT", OwnT mr_tgt1);
+                                      ("X", ((R a1 mp_src1 mp_tgt1 ** FR) ∧ Exactly rx1)%I)]),
+            gpaco8 (_sim_itree (mk_wf R) le) (cpn8 (_sim_itree (mk_wf R) le)) rg rg _ _ eqr o_new_src o_new_tgt _a
+                   (Any.pair mp_src1 mr_src1↑, k_src (ctx1, tt))
+                   (Any.pair mp_tgt1 mr_tgt1↑, k_tgt (ctx1 ⋅ rx1, tt)))
+    :
+      gpaco8 (_sim_itree (mk_wf R) le) (cpn8 (_sim_itree (mk_wf R) le)) r rg _ _ eqr o_src0 o_tgt0 _a
+             (Any.pair mp_src0 mr_src0↑, (interp_hCallE_tgt mn stb_src d APC ctx0) >>= k_src)
+             (Any.pair mp_tgt0 mr_tgt0↑, (interp_hCallE_tgt mn stb_tgt d APC (ctx0 ⋅ rx0)) >>= k_tgt)
+  .
+  Proof.
+    subst.
+    unfold APC. steps. force_l. exists x. steps. force_l; ss. steps.
+
+    (* Unset Printing Notations. *)
+    instantiate (1:=5%ord). instantiate (1:=5%ord).
+    clear_until x. gen x d ctx0 rx0. gen mp_src0 mp_tgt0 mr_src0 mr_tgt0. gen a0. gen Xtra. gcofix CIH. i.
+    {
+      rewrite unfold_APC. ired_both.
+      force_r. i. force_l. exists x0.
+      destruct x0.
+      - steps. eapply gpaco8_mon; et.
+        { eapply ARG.
+          { refl. }
+          clear - ACC ENTAIL.
+          eapply current_iPropL_pop in ACC; des.
+          eapply current_iPropL_pop in TL; des.
+          eapply current_iPropL_nil in TL0. ss.
+          eapply current_iPropL_push; et.
+          uipropall. des. clarify.
+          exploit ENTAIL; try apply HD0.
+          { eapply wf_extends; et. r. exists (ctx0 ⋅ hdr). r_solve. }
+          i; des. clarify.
+          eapply current_iPropL_push; cycle 1.
+          { ss. esplits; et. }
+          eapply current_iPropL_nil.
+          { r_wf TL0. }
+        }
+      -
+        assert(T: exists rf_src rm_src, R a0 mp_src0 mp_tgt0 rm_src /\ FR rf_src /\ rx0 = rf_src ⋅ rm_src).
+        { clear - ACC ENTAIL. uipropall.
+          eapply current_iPropL_pop in ACC. des.
+          eapply current_iPropL_pop in TL. des.
+          eapply current_iPropL_nil in TL0. ss.
+          des. clarify.
+          exploit ENTAIL; try apply HD0.
+          { eapply wf_extends; et. exists (ctx0 ⋅ hdr). r_solve. }
+          i; des. clarify. esplits; et.
+          r_solve.
+        }
+        des. subst.
+
+        steps. force_l. exists x0. steps. force_l; ss. steps. unfold HoareCall. unfold mput, mget. steps.
+        des; ss.
+        assert(STB: stb_src s = Some f).
+        { eapply STBINCL; et. r. esplits; et. }
+        force_l. eexists (_, _). steps. rewrite STB. steps. instantiate (1:=t).
+        unfold HoareCall. unfold mput, mget. steps.
+
+        force_l. rename c into mr_tgt1. rename c0 into ro. rename c1 into rf.
+        exists (ro, rf ⋅ rf_src, rm_src ⋅ mr_tgt1). steps. force_l; ss.
+        { r_wf _GUARANTEE1. }
+        steps. force_l. esplits; et. steps. force_l. esplits; et. steps. force_l. esplits; et.
+        steps. force_l; et. steps. force_l; ss. steps.
+        { econs. eapply to_semantic. iIntros "[A B]". iFrame. iStopProof.
+          uipropall. i. r in H0. des; clarify. esplits; et. r. uipropall.
+        }
+
+        inv WF. rewrite Any.pair_split in *. clarify. rewrite Any.upcast_downcast. steps.
+        hexploit1 RSRC.
+        { eapply wf_extends; et. r. exists (c ⋅ rf ⋅ rf_src ⋅ c0). r_solve. }
+        rename c into ri. rename c0 into ctx1.
+        r in RSRC. autounfold with iprop in RSRC; autorewrite with iprop in RSRC. des. clarify.
+        rename a into rinv.
+        force_r. exists (ri, ctx1 ⋅ (rinv ⋅ rf_src)). steps. force_r; ss.
+        { eapply wf_extends; et.
+          Local Transparent OwnT. r in RSRC1. uipropall. r in RSRC1. des; clarify.
+          r. exists (ctx). r_solve. }
+        steps. force_r. esplits. steps. force_r; et. steps.
+
+        move CIH at bottom.
+        gbase. eapply (CIH _ w1); et.
+        { i. eapply ARG; try apply ACC0. etrans; et. }
+        { eapply current_iPropL_push; et.
+          eapply current_iPropL_push; cycle 1.
+          { ss. uipropall. unfold Exactly. uipropall. esplits; et. }
+          eapply current_iPropL_nil.
+          eapply wf_extends; try apply _ASSUME.
+          exists (ri ⋅ rf). r_solve.
+        }
+    }
+  Unshelve. all: try exact 0.
+  Qed.
+
 End MODE.
 
 Global Opaque OwnT.
@@ -727,6 +867,16 @@ Tactic Notation "hret" uconstr(a) :=
   |i; iIntros "Q"
   ].
 
+Tactic Notation "hAPC" uconstr(a) :=
+  eapply (hAPC_both _ a);
+  [refl
+  |refl
+  |try (typeclasses eauto)
+  |eassumption
+  |
+  |
+  |on_current ltac:(fun H => try clear H); i; on_current ltac:(fun H => simpl in H)]
+.
 
 
 
